Lambda/Combinators.v
@@ -12,6 +12,8 @@ Require Import Arith.
 
 Notation "x =? y" := (dec x y) (at level 70).
 
+(** * Syntax of terms *)
+
 Inductive Term : Type :=
     | Var : V -> Term
     | K : Term
@@ -19,6 +21,8 @@ Inductive Term : Type :=
     | App : Term -> Term -> Term.
 
 Notation "M @ N" := (App M N) (at level 50, left associativity).
+
+(** * Reduction relation *)
 
 Inductive WStep : Term -> Term -> Prop :=
     | WStep_K :
@@ -33,23 +37,20 @@ Inductive WStep : Term -> Term -> Prop :=
         forall A B B' : Term,
           WStep B B' -> WStep (App A B) (App A B').
 
-Hint Constructors WStep.
-
 Notation "A ~> B" := (WStep A B) (at level 60).
 
 Inductive WSteps : Term -> Term -> Prop :=
-(*    | WSteps_WStep :
-        forall A B : Term, WStep A B -> WSteps A B*)
     | WSteps_refl :
         forall A : Term, WSteps A A
     | WSteps_trans :
         forall A B C : Term, WStep A B -> WSteps B C -> WSteps A C.
 
-Hint Constructors WSteps.
-
 Notation "A ~>* B" := (WSteps A B) (at level 60).
 
-(*
+Hint Constructors WStep WSteps : core.
+
+(** * Properties of reduction *)
+
 Require Import Relation_Definitions Setoid Morphisms.
 
 Instance WStep_WSteps_L :
@@ -71,15 +72,6 @@ Instance WStep_WSteps :
 Proof.
   unfold Proper, respectful. intros A A' HA B B' HB. eauto.
 Qed.
-
-Instance WStep_WSteps' :
-  Proper (WStep ==> WStep ==> Basics.flip Basics.impl) WSteps.
-Proof.
-  unfold Proper, respectful. intros A A' HA B B' HB.
-  unfold Basics.flip, Basics.impl. intro.
-  induction H.
-Qed.
-*)
 
 Lemma WSteps_trans' :
   forall {A B C : Term},
@@ -111,6 +103,9 @@ Proof.
     eauto.
 Qed.
 
+(** * Derived combinators *)
+
+(** Identity *)
 Definition I : Term := S @ K @ K.
 
 Lemma WStep_I :
@@ -119,7 +114,9 @@ Proof.
   intros. unfold I. eauto.
 Defined.
 
-Hint Resolve WStep_I.
+Hint Resolve WStep_I : core.
+
+(** * Lambdas *)
 
 Fixpoint lam (x : V) (A : Term) : Term :=
 match A with
@@ -136,12 +133,6 @@ match A with
     | S => S
     | A1 @ A2 => subst x A1 B @ subst x A2 B
 end.
-
-(*
-Lemma WStep_L :
-  forall {A A' B : Term},
-    A ~> A' -> A @ B 
-*)
 
 Lemma lam_WSteps :
   forall (x : V) (A : Term),
@@ -167,18 +158,270 @@ Proof.
       apply WSteps_App; auto.
 Qed.
 
-Parameter v : V.
+(** * Normal forms *)
 
-Definition pair (A B : Term) : Term := lam v (Var v @ A @ B).
+Inductive Nf : Term -> Prop :=
+    | Nf_K   : Nf K
+    | Nf_S   : Nf S
+    | Nf_Kt  : forall t : Term, Nf t -> Nf (K @ t)
+    | Nf_St  : forall t : Term, Nf t -> Nf (S @ t)
+    | Nf_Stt : forall t1 t2 : Term, Nf t1 -> Nf t2 -> Nf (S @ t1 @ t2)
+    | Nf_Ne  : forall t : Term, Ne t -> Nf t
 
-Definition outL (A : Term) : Term := A @ K.
+with Ne : Term -> Prop :=
+    | Ne_var : forall v : V, Ne (Var v)
+    | Ne_App : forall t1 t2 : Term, Ne t1 -> Nf t2 -> Ne (App t1 t2).
 
-Definition outR (A : Term) : Term := A @ (K @ I).
+Ltac inv H := inversion H; subst; clear H.
 
-Lemma outL_pair :
-  forall A B : Term, outL (pair A B) ~>* A.
+Lemma Nf_spec :
+  forall t : Term, Nf t <-> (forall t' : Term, ~ WStep t t').
 Proof.
-  unfold outL, pair. intros. eapply WSteps_trans'.
-    apply lam_subst.
-    cbn. destruct (dec_spec v v).
-Abort.
+  split.
+    induction t; intros Hnf t' Hred.
+      inv Hred.
+      inv Hred.
+      inv Hred.
+      inv Hred.
+        inv Hnf. inv H. inv H2. inv H1.
+        inv Hnf. inv H. inv H2. inv H1. inv H2.
+        eapply IHt1.
+          inv Hnf.
+            inv H2.
+            inv H2.
+            constructor. assumption.
+            inv H. constructor. assumption.
+          eassumption.
+        eapply IHt2.
+          inv Hnf; try inv H; assumption.
+          eassumption.
+    induction t; intros.
+      do 2 constructor.
+      constructor.
+      constructor.
+      destruct t1.
+        do 2 constructor.
+          constructor.
+          apply IHt2. do 2 intro. eapply H.
+            apply WStep_AppR. eassumption.
+        constructor. apply IHt2. do 2 intro. eapply H. eauto.
+        constructor. apply IHt2. do 2 intro. eapply H. eauto.
+      destruct t1_1.
+        do 2 constructor.
+          constructor.
+            constructor.
+            cut (Nf (Var v @ t1_2)).
+              intro. inv H0. inv H1. assumption.
+              apply IHt1. do 2 intro. eapply H. eauto.
+          apply IHt2. do 2 intro. eapply H. eauto.
+          specialize (H t1_2). contradict H. constructor.
+          constructor.
+            assert (Nf (S @ t1_2)).
+              apply IHt1. do 2 intro. inv H0.
+                inv H4.
+                eapply H. eauto.
+              inv H0.
+                assumption.
+                inv H1. inv H3.
+            apply IHt2. do 2 intro. eapply H. eauto.
+          constructor. constructor.
+            assert (Nf (t1_1_1 @ t1_1_2 @ t1_2)).
+              apply IHt1. do 2 intro. eapply H. eauto.
+              inv H0.
+                specialize (H (t1_1_2 @ t2 @ (t1_2 @ t2))).
+                  contradict H. constructor.
+                assumption.
+            apply IHt2. do 2 intro. eapply H. eauto.
+Qed.
+
+(*
+Require Import Equality.
+
+Fixpoint isProp_Nf
+  (isProp_Term : forall (t1 t2 : Term) (p q : t1 = t2), p = q) (t : Term) {struct t}
+    : forall nf1 nf2 : Nf t, nf1 = nf2
+
+with isProp_Ne
+  (isProp_Term : forall (t1 t2 : Term) (p q : t1 = t2), p = q) (t : Term) {struct t}
+    : forall ne1 ne2 : Ne t, ne1 = ne2.
+Proof.
+  destruct t; intros.
+    dependent destruction nf1. dependent destruction nf2.
+      f_equal. dependent destruction n. dependent destruction n0. reflexivity.
+    dependent destruction nf1.
+      dependent destruction nf2.
+        reflexivity.
+        inv n.
+      inv n.
+    dependent destruction nf1.
+      dependent destruction nf2.
+        reflexivity.
+        inv n.
+      inv n.
+    dependent destruction nf1.
+      dependent destruction nf2.
+        f_equal. apply isProp_Nf. assumption.
+        exfalso. inv n. inv H1.
+      dependent destruction nf2.
+        f_equal. apply isProp_Nf. assumption.
+        exfalso. inv n. inv H1.
+      dependent destruction nf2.
+        f_equal.
+          apply isProp_Nf. assumption.
+          apply isProp_Nf. assumption.
+        exfalso. inv n. inv H1. inv H3.
+      dependent destruction nf2.
+        exfalso. inv n. inv H1.
+        exfalso. inv n. inv H1.
+        exfalso. inv n. inv H1. inv H3.
+        f_equal. apply isProp_Ne. assumption.
+  destruct t; intros.
+    dependent destruction ne1. dependent destruction ne2.
+      reflexivity.
+    dependent destruction ne1.
+    dependent destruction ne1.
+    dependent destruction ne1. dependent destruction ne2. f_equal.
+      apply isProp_Ne. assumption.
+      apply isProp_Nf. assumption.
+Qed.
+*)
+
+Print WStep.
+
+Inductive parallel : Term -> Term -> Prop :=
+    | parallel_K :
+        forall t1 t2 : Term,
+          parallel (K @ t1 @ t2) t1
+    | parallel_S :
+        forall t1 t2 t3 : Term,
+          parallel (S @ t1 @ t2 @ t3) (t1 @ t3 @ (t2 @ t3))
+    | parallel_AppL :
+        forall t1 t1' t2 : Term,
+          parallel t1 t1' -> parallel (t1 @ t2) (t1' @ t2)
+    | parallel_AppR :
+        forall t1 t2 t2' : Term,
+          parallel t2 t2' -> parallel (t1 @ t2) (t1 @ t2')
+    | parallel_App :
+        forall t1 t1' t2 t2' : Term,
+          parallel t1 t1' -> parallel t2 t2' -> parallel (t1 @ t2) (t1' @ t2').
+
+Hint Constructors parallel : core.
+
+Require Import FormalSystems.Base.
+
+Definition parallels := rtc parallel.
+
+Hint Unfold parallels : core.
+
+Lemma parallels_K :
+  forall t1 t2 : Term,
+    parallels (K @ t1 @ t2) t1.
+Proof.
+  do 2 constructor.
+Qed.
+
+Lemma parallels_S :
+  forall t1 t2 t3 : Term,
+    parallels (S @ t1 @ t2 @ t3) (t1 @ t3 @ (t2 @ t3)).
+Proof.
+  do 2 constructor.
+Qed.
+
+Lemma parallels_AppL :
+  forall t1 t1' t2 : Term,
+    parallels t1 t1' -> parallels (t1 @ t2) (t1' @ t2).
+Proof.
+  unfold parallels.
+  intros until 1. revert t2.
+  induction H; eauto.
+Qed.
+
+Lemma parallels_AppR :
+  forall t1 t2 t2' : Term,
+    parallels t2 t2' -> parallels (t1 @ t2) (t1 @ t2').
+Proof.
+  unfold parallels.
+  intros until 1. revert t1.
+  induction H; eauto.
+Qed.
+
+Hint Resolve parallels_K parallels_S parallels_AppL parallels_AppR : core.
+
+Hint Extern 0 =>
+  match goal with
+    | |- parallels (K @ _ @ _) _ => try apply parallels_K
+  end.
+
+Lemma parallels_App :
+  forall t1 t1' t2 t2' : Term,
+    parallels t1 t1' -> parallels t2 t2' ->
+      parallels (t1 @ t2) (t1' @ t2').
+Proof.
+  unfold parallels.
+  intros until 1. revert t2 t2'.
+  induction H; intros.
+    econstructor 3.
+      do 2 constructor; eauto.
+      induction H0; eauto.
+    apply parallels_AppR. assumption.
+    eapply rtc_trans.
+      apply IHrtc1. eassumption.
+      apply IHrtc2. constructor 2.
+Qed.
+
+Lemma parallel_confluent :
+  forall a b c : Term,
+    parallel a b -> parallel a c ->
+      exists d : Term, parallels b d /\ parallels c d.
+Proof.
+  intros a b c Hpb Hpc.
+  revert c Hpc.
+  induction Hpb; intros; unfold parallels in *.
+    inv Hpc; eauto.
+      inv H2; eauto.
+        inv H3.
+        inv H1.
+      inv H1; eauto.
+        inv H4.
+        inv H2.
+    inv Hpc; eauto.
+      inv H2; eauto.
+        inv H3; eauto.
+          inv H2. exists (t2' @ t3 @ (t2 @ t3)). auto.
+          inv H1.
+        exists (t1 @ t3 @ (t2' @ t3)). auto.
+        inv H1; eauto.
+          inv H3.
+          exists (t2'0 @ t3 @ (t2' @ t3)). auto.
+          inv H2.
+      exists (t1 @ t2' @ (t2 @ t2')). auto.
+      inv H1; eauto.
+        inv H4; eauto.
+          inv H2.
+          exists (t2'0 @ t2' @ (t2 @ t2')). auto.
+          inv H1.
+        exists (t1 @ t2' @ (t2'0 @ t2')). auto.
+        inv H2.
+          inv H4.
+          exists (t2'1 @ t2' @ (t2'0 @ t2')). auto.
+          inv H1.
+    inv Hpc; eauto.
+      inv Hpb; eauto.
+        inv H2.
+        inv H1.
+      inv Hpb; eauto.
+        inv H2; eauto.
+          inv H3.
+          exists (t2' @ t2 @ (t3 @ t2)). auto.
+          inv H1.
+        exists (t0 @ t2 @ (t2' @ t2)). auto.
+        inv H1; eauto.
+          inv H4.
+          exists (t2'0 @ t2 @ (t2' @ t2)). auto.
+          inv H2.
+      decompose [ex and] (IHHpb _ H2). exists (x @ t2). split.
+        apply parallels_AppL. assumption.
+        apply parallels_AppL. assumption.
+      exists (t1' @ t2'). auto.
+      decompose [ex and] (IHHpb _ Hpb). decompose [ex and] (IHHpb _ H1).
+Abort.       
