Lambda/LambdaCalculus.v
@@ -12,21 +12,73 @@ Require Import Arith.
 
 Notation "x =? y" := (dec x y) (at level 70).
 
-Inductive Term : Type :=
-    | Var : V -> Term
-    | Lam : (V -> Term) -> Term
-    | App : Term -> Term -> Term.
+Inductive Term (Var : Type) : Type :=
+    | Var : Var -> Term Var
+    | Lam : (Var -> Term Var) -> Term Var
+    | App : Term Var -> Term Var -> Term Var.
 
-Fixpoint subst (M : Term) (x : V) (N : Term) : Term :=
-match M with
-    | Var v => if x =? v then N else Var v
-    | Lam M' => Lam (fun v : V => (subst (M' v) x N))
-    | App P Q => App (subst P x N) (subst P x Q)
+Definition Term' : Type := forall Var : Type, Term Var.
+
+Arguments Var {Var} _.
+Arguments Lam {Var} _.
+Arguments App {Var} _ _.
+
+Fixpoint numOfVars (t : Term unit) : nat :=
+match t with
+    | Var _ => 1
+    | Lam t' => numOfVars (t' tt)
+    | App t1 t2 => numOfVars t1 + numOfVars t2
 end.
 
-(* TODO: it's high time to learn PHOAS properly *)
+Fixpoint subst' {A : Type} (M : Term (Term A)) : Term A :=
+match M with
+    | Var v => v
+    | Lam M' => Lam (fun x : A => subst' (M' (Var x)))
+    | App P Q => App (subst' P) (subst' Q)
+end.
+
+Definition subst
+  (M : forall A : Type, A -> Term A) (N : Term') : Term' :=
+    fun A : Type => subst' (M (Term A) (N A)).
+
+Compute
+  subst (fun A x => App (Var x) (Var x)) (fun A => Lam (fun x : A => Var x)).
+
 (*
-Inductive Beta : Term -> Term -> Prop :=
+Inductive Beta {A : Type} : Term A -> Term A -> Prop :=
     | BetaContraction :
-        forall (M : V -> Term) (N : Term), Beta (App (Lam M) N)
+        forall (M : A -> Term A) (N : Term A),
+          Beta (App (Lam M) N) 
+    | BetaAppL :
+        forall P P' Q : Term',
+          Beta P P' ->
+            Beta (fun A => App (P A) (Q A)) (fun A => App (P' A) (Q A))
+    | BetaAppR :
+        forall P Q Q' : Term',
+          Beta Q Q' ->
+            Beta (fun A => App (P A) (Q A)) (fun A => App (P A) (Q' A))
+    | BetaLam :
+        forall M M' : forall A : Type, A -> Term A,
+          Beta M M' ->
+          Beta (fun A => Lam (M A)) (fun A => Lam (M' A)).
+*)
+
+(*
+Inductive Beta : Term' -> Term' -> Prop :=
+    | BetaContraction :
+        forall (M : forall A : Type, A -> Term A) (N : Term'),
+          Beta (fun A => App (Lam (M A)) (N A)) (fun A => subst M N A)
+    | BetaAppL :
+        forall P P' Q : Term',
+          Beta P P' ->
+            Beta (fun A => App (P A) (Q A)) (fun A => App (P' A) (Q A))
+    | BetaAppR :
+        forall P Q Q' : Term',
+          Beta Q Q' ->
+            Beta (fun A => App (P A) (Q A)) (fun A => App (P A) (Q' A))
+    | BetaLam :
+        forall M M' : forall A : Type, A -> Term A,
+          (forall x : (forall A : Type, Term A),
+            Beta (fun A => M (Term A) (x A)) (fun A => M' (Term A) (x A))) ->
+          Beta (fun A => Lam (M A)) (fun A => Lam (M' A)).
 *)
