CoL/coindcoind.v
@@ -1,0 +1,25 @@
+(*
+
+  If there was anything like coinduction-coinduction in Coq, this is how we
+  would use it to define Constant Games together with their Winners at the
+  same time.
+
+CoInductive ConstantGame : Type :=
+{
+    winner : Player;
+    Labmove : Type;
+    who : Labmove -> Player;
+    next : Labmove -> ConstantGame;
+}
+
+with Winner (g : ConstantGame) (p : Player) : Prop :=
+{
+    Winner0 : (Labmove g -> False) -> p = winner g;
+    Winner1 :
+      Labmove g ->
+        (exists move : Labmove g,
+          who g move = p /\ Winner (next g move) p) \/
+        (forall move : Labmove g,
+          who g move = swap p -> Winner (next g move) p);
+}.
+*)
